theories/RTL/SimRules.v
@@ -18,236 +18,385 @@ Section Rules.
 
   Abbreviation fsim := (fsim WfNat WfNat Pₜ Pₛ).
   Abbreviation fsim_lfp := (fsim_lfp WfNat WfNat Pₜ Pₛ).
-  Abbreviation rlogic := (rlogic _ _).
+  Abbreviation post := (val -> val -> rlogic).
 
-  Definition sim GFP Q (stepₜ: nat) fₜ pcₜ (stepₛ: nat) fₛ pcₛ : rlogic :=
-    let sim_rtl Φ : rlogic :=
-      (fun ρₜ ρₛ mₜ mₛ =>
-         fsim_lfp GFP Φ
-           stepₜ ([], State fₜ pcₜ ρₜ, mₜ)
-           stepₛ ([], State fₛ pcₛ ρₛ, mₛ))
+  Implicit Types C : Chain fsim_lfp.
+
+  Definition sim C Γ Φ fₜ pcₜ j i fₛ pcₛ : rlogic :=
+    let Φ : value Λₜ -> value Λₛ -> Prop :=
+      fun '(vₜ, mₜ) '(vₛ, mₛ) => Φ vₜ vₛ mₜ mₛ
     in
-    ⦇ ∀ Φ,
-        ⌜∀ vₜ vₛ mₜ mₛ, Q vₜ vₛ mₜ mₛ -> Φ (vₜ, mₜ) (vₛ, mₛ)⌝ ->
-        sim_rtl Φ ⦈.
+    let '(ρₜ, ρₛ) := Γ in
+    fun mₜ mₛ =>
+      fsim_lfp (elem C) Φ
+        j ([], State fₜ pcₜ ρₜ, mₜ)
+        i ([], State fₛ pcₛ ρₛ, mₛ).
 
   Notation
-    "C ⊢ '⟨' ft '@' pct ',' j '⟩' '≲' '⟨' fs '@' pcs ',' i '⟩' '{{' Φ '}}'" :=
-    (sim (elem C) Φ j ft pct i fs pcs)
+    "C '|' Γ '⊢' ft '@' pct  '<{' j ',' i '}=' fs '@' pcs '{{' Φ '}}'" :=
+    (sim C Γ Φ%rlogic ft pct j i fs pcs)
       (at level 1, ft at level 0, fs at level 0, no associativity).
 
-  Lemma both_ret (C : Chain fsim_lfp) Q j fₜ pcₜ i fₛ pcₛ :
+  Definition hoare C Γ P fₜ pcₜ j i fₛ pcₛ (Q: post) : Prop :=
+    ⊨ ∀ Φ,
+      P -*
+      (∀ vₜ vₛ, Q vₜ vₛ -* Φ vₜ vₛ) -*
+      sim C Γ Φ fₜ pcₜ j i fₛ pcₛ.
+
+  Notation
+    "C '|' Γ '⊢' '{{' P '}}' ft '@' pct  '<{' j ',' i '}=' fs '@' pcs '{{' Q '}}'" :=
+    (hoare C Γ P%rlogic ft pct j i fs pcs Q%rlogic)
+      (at level 1, ft at level 0, fs at level 0, no associativity).
+
+  Lemma both_ret C Γ (Φ: post)  fₜ pcₜ j i fₛ pcₛ :
     ∀ rₜ vₜ rₛ vₛ,
-    fₜ@pcₜ is <{ ret rₜ }> ->
-    fₛ@pcₛ is <{ ret rₛ }> ->
-    ⊨ rₜ ⇒ₜ vₜ ->
-      rₛ ⇒ₛ vₛ ->
-      ⌜Q vₜ vₛ⌝ₘ ->
-      C ⊢ ⟨fₜ @ pcₜ, j⟩ ≲ ⟨fₛ @ pcₛ, i⟩ {{ Q }}.
+    fₜ@pcₜ is <<{ ret rₜ }>> ->
+    fₛ@pcₛ is <<{ ret rₛ }>> ->
+    Γ @ rₜ ⇒ₜ vₜ ->
+    Γ @ rₛ ⇒ₛ vₛ ->
+    C | Γ ⊢ {{ Φ vₜ vₛ }} fₜ @ pcₜ <{j, i}= fₛ @ pcₛ {{ Φ }}.
   Proof using Type.
-    intros rt vt rs vs Hpct Hpcs.
-    intros ρₜ ρₛ mₜ mₛ Ht Hs HQ Ψ Hpost. simp.
+    intros rt vt rs vs Hpct Hpcs Ht Hs.
+    intros Ψ mt1 ms1 ? ? Hpre mt2 ms2 ? ? Hpost.
+
+    simp. decompose_map_disjoint.
+    destruct Γ as [ρₜ ρₛ].
+    unfold rbank_assert_t, rbank_assert_t_single in Ht.
+    unfold rbank_assert_s, rbank_assert_s_single in Hs.
+
     eapply FSourceSteps with (i' := 0).
-    { econstructor; eassumption || reflexivity. }
+    { eapply exec_Iret; eassumption. }
+
     eapply FTargetSteps.
-    { eexists; econstructor; eassumption || reflexivity. }
-    intros t' Hstep. inv Hstep.
-    exists 0.
-    eapply FBothFinal.
-    do 2 econstructor. repeat split.
-    now apply Hpost.
+    { eexists; eapply exec_Iret; eassumption. }
+
+    intros t' Hstep. inv Hstep. exists 0.
+
+    eapply FRelated.
+
+    do 2 eexists; repeat split. simpl.
+
+    rewrite (map_empty_union mt1).
+    rewrite (map_empty_union ms1).
+
+    erewrite (map_union_comm mt1 mt2) by eauto.
+    erewrite (map_union_comm ms1 ms2) by eauto.
+    apply Hpost.
+    - solve_map_disjoint.
+    - solve_map_disjoint.
+    - apply Hpre.
   Qed.
 
-  Lemma source_nop (C : Chain fsim_lfp) Q j fₜ pcₜ i fₛ pcₛ :
+  Lemma source_nop C Γ Φ j fₜ pcₜ i fₛ pcₛ :
     ∀ pc,
-    fₛ@pcₛ is <{ nop -> pc }> ->
-    ⊨ C ⊢ ⟨fₜ @ pcₜ, j⟩ ≲ ⟨fₛ @ pc, S i⟩ {{ Q }} ->
-      C ⊢ ⟨fₜ @ pcₜ, j⟩ ≲ ⟨fₛ @ pcₛ, i⟩ {{ Q }}.
+    fₛ@pcₛ is <<{ nop -> pc }>> ->
+    C | Γ ⊢ {{ ⌜⌝ }} fₜ @ pcₜ <{j, 1+i}= fₛ @ pc {{ Φ }} ->
+    C | Γ ⊢ {{ ⌜⌝ }} fₜ @ pcₜ <{j, i}= fₛ @ pcₛ {{ Φ }}.
   Proof using Type.
-    intros pc Hpc.
-    intros ρₜ ρₛ mₜ mₛ H Ψ Hpost. simp.
+    intros pc Hpc H.
+    intros Ψ mt1 ms1 ? ? Hpre mt2 ms2 ? ? Hpost.
+
+    simp.
+    destruct Γ as [ρₜ ρₛ].
+
     eapply FSourceSteps.
-    - constructor; eassumption.
+    - econstructor; eassumption.
     - now apply H.
   Qed.
 
-  Lemma target_nop (C : Chain fsim_lfp) Q j fₜ pcₜ i fₛ pcₛ :
+  Lemma target_nop C Γ Φ j fₜ pcₜ i fₛ pcₛ :
     ∀ pc,
-    fₜ@pcₜ is <{ nop -> pc }> ->
-    ⊨ C ⊢ ⟨fₜ @ pc, S j⟩ ≲ ⟨fₛ @ pcₛ, i⟩ {{ Q }} ->
-      C ⊢ ⟨fₜ @ pcₜ, j⟩ ≲ ⟨fₛ @ pcₛ, i⟩ {{ Q }}.
+    fₜ@pcₜ is <<{ nop -> pc }>> ->
+    C | Γ ⊢ {{ ⌜⌝ }} fₜ @ pc <{1+j, i}= fₛ @ pcₛ {{ Φ }} ->
+    C | Γ ⊢ {{ ⌜⌝ }} fₜ @ pcₜ <{j, i}= fₛ @ pcₛ {{ Φ }}.
   Proof using Type.
-    intros pc Hpc.
-    intros ρₜ ρₛ mₜ mₛ H Ψ Hpost. simp.
+    intros pc Hpc H.
+    intros Ψ mt1 ms1 ? ? Hpre mt2 ms2 ? ? Hpost.
+
+    simp.
+    destruct Γ as [ρₜ ρₛ].
+
     eapply FTargetSteps.
-    - eexists. constructor; eassumption.
+    - eexists. econstructor; eassumption.
     - intros t Hstep. inv Hstep.
       eexists. now apply H.
   Qed.
 
-  Lemma mapMtoMap {A B : Type} : ∀ (f : A -> B) args,
-    mapM (fun x => Some (f x)) args = Some (map f args).
-  Proof using Type.
-    intros f args.
-    induction args as [ | hd tl IH ].
-    - reflexivity.
-    - simpl. now rewrite IH.
-  Qed.
-
-  Lemma source_op (C : Chain fsim_lfp) Q j fₜ pcₜ i fₛ pcₛ :
+  Lemma source_op C Γ Φ j fₜ pcₜ i fₛ pcₛ :
     ∀ pc dst op regs args v,
-    fₛ@pcₛ is <{ dst := @op regs -> pc }> ->
+    fₛ@pcₛ is <<{ dst := @op regs -> pc }>> ->
     eval_op op args = Some v ->
-    ⊨ regs ⇒ₛ args ->
-      ⟦ dst ⇐ₛ v ⟧ C ⊢ ⟨fₜ @ pcₜ, j⟩ ≲ ⟨fₛ @ pc, S i⟩ {{ Q }} ->
-      C ⊢ ⟨fₜ @ pcₜ, j⟩ ≲ ⟨fₛ @ pcₛ, i⟩ {{ Q }}.
+    Γ @ regs ⇒ₛ args ->
+    C | ⟦ dst ⇐ₛ v ⟧Γ ⊢ {{ ⌜⌝ }} fₜ @ pcₜ <{j, 1+i}= fₛ @ pc {{ Φ }} ->
+    C | Γ ⊢ {{ ⌜⌝ }} fₜ @ pcₜ <{j, i}= fₛ @ pcₛ {{ Φ }}.
   Proof using Type.
-    intros pc dst op regs args v Hpc Hv.
-    intros ρₜ ρₛ mₜ mₛ Harg [? [Hnew Hsim]] Ψ Hpost. simp.
+    intros pc dst op regs args v Hpc Hv Hargs H.
+    intros Ψ mt1 ms1 ? ? Hpre mt2 ms2 ? ? Hpost.
 
-    rewrite mapMtoMap in Harg.
-    injection Harg as Harg.
-
-    injection Hnew as Hnew.
+    simp.
+    destruct Γ as [ρₜ ρₛ].
 
     eapply FSourceSteps.
     - econstructor; eassumption || reflexivity.
-    - now apply Hsim.
+    - now eapply H.
   Qed.
 
-  Lemma target_op (C : Chain fsim_lfp) Q j fₜ pcₜ i fₛ pcₛ :
+  Lemma target_op C Γ Φ j fₜ pcₜ i fₛ pcₛ :
     ∀ pc dst op regs args v,
-    fₜ@pcₜ is <{ dst := @op regs -> pc }> ->
+    fₜ@pcₜ is <<{ dst := @op regs -> pc }>> ->
     eval_op op args = Some v ->
-    ⊨ regs ⇒ₜ args ->
-      ⟦ dst ⇐ₜ v ⟧ C ⊢ ⟨fₜ @ pc, S j⟩ ≲ ⟨fₛ @ pcₛ, i⟩ {{ Q }} ->
-      C ⊢ ⟨fₜ @ pcₜ, j⟩ ≲ ⟨fₛ @ pcₛ, i⟩ {{ Q }}.
+    Γ @ regs ⇒ₜ args ->
+    C | ⟦ dst ⇐ₜ v ⟧Γ ⊢ {{ ⌜⌝ }} fₜ @ pc <{1+j, i}= fₛ @ pcₛ {{ Φ }} ->
+    C | Γ ⊢ {{ ⌜⌝ }} fₜ @ pcₜ <{j, i}= fₛ @ pcₛ {{ Φ }}.
   Proof using Type.
-    intros pc dst op regs args v Hpc Hv.
-    intros ρₜ ρₛ mₜ mₛ Harg [? [Hnew Hsim]] Ψ Hpost. simp.
+    intros pc dst op regs args v Hpc Hv Hargs H.
+    intros Ψ mt1 ms1 ? ? Hpre mt2 ms2 ? ? Hpost.
 
-    rewrite mapMtoMap in Harg.
-    injection Harg as Harg.
-
-    injection Hnew as Hnew.
+    simp.
+    destruct Γ as [ρₜ ρₛ].
+    unfold rbank_assert_t, rbank_assert_t_list in Hargs.
 
     eapply FTargetSteps.
     - eexists. econstructor; eassumption || reflexivity.
     - intros t Hstep. inv Hstep.
-      eexists. now apply Hsim.
+      eexists. now apply H.
   Qed.
 
-  Lemma source_load (C : Chain fsim_lfp) Q j fₜ pcₜ i fₛ pcₛ :
+  Lemma source_load C Γ Φ j fₜ pcₜ i fₛ pcₛ :
     ∀ pc dst src addr v,
-    fₛ@pcₛ is <{ dst := !src -> pc }> ->
-    ⊨ src ⇒ₛ addr ->
-      addr →ₛ v ->
-      ⟦ dst ⇐ₛ v ⟧ C ⊢ ⟨fₜ @ pcₜ, j⟩ ≲ ⟨fₛ @ pc, S i⟩ {{ Q }} ->
-      C ⊢ ⟨fₜ @ pcₜ, j⟩ ≲ ⟨fₛ @ pcₛ, i⟩ {{ Q }}.
+    fₛ@pcₛ is <<{ dst := !src -> pc }>> ->
+    Γ @ src ⇒ₛ addr ->
+    C | ⟦ dst ⇐ₛ v ⟧Γ ⊢ {{ addr →ₛ v }} fₜ @ pcₜ <{j, 1+i}= fₛ @ pc {{ Φ }} ->
+    C | Γ ⊢ {{ addr →ₛ v }} fₜ @ pcₜ <{j, i}= fₛ @ pcₛ {{ Φ }}.
   Proof using Type.
-    intros pc dst src addr v Hpc.
-    intros ρₜ ρₛ mₜ mₛ Hsrc Haddr [? [Hnew Hsim]] Ψ Hpost. simp.
+    intros pc dst src addr v Hpc Haddr H.
+    intros Ψ mt1 ms1 ? ? Hpre mt2 ms2 ? ? Hpost.
 
-    injection Hsrc as Hsrc.
-    injection Hnew as Hnew.
+    simp.
+    destruct Γ as [ρₜ ρₛ].
+    apply get_at_unfold in Hpre. destruct Hpre as (loc & Hloc & Hget).
+
+    eapply FSourceSteps.
+    - eapply exec_Iload; try eassumption.
+      + unfold get_at. rewrite Hloc. simpl_map. reflexivity.
+      + reflexivity.
+    - apply H; auto.
+      unfold get_at. now rewrite Hloc.
+  Qed.
+
+  Lemma target_load C Γ Φ j fₜ pcₜ i fₛ pcₛ :
+    ∀ pc dst src addr v,
+    fₜ@pcₜ is <<{ dst := !src -> pc }>> ->
+    Γ @ src ⇒ₜ addr ->
+    C | ⟦ dst ⇐ₜ v ⟧Γ ⊢ {{ addr →ₜ v }} fₜ @ pc <{1+j, i}= fₛ @ pcₛ {{ Φ }} ->
+    C | Γ ⊢ {{ addr →ₜ v }} fₜ @ pcₜ <{j, i}= fₛ @ pcₛ {{ Φ }}.
+  Proof using Type.
+    intros pc dst src addr v Hpc Haddr H.
+    intros Ψ mt1 ms1 ? ? Hpre mt2 ms2 ? ? Hpost.
+
+    destruct Γ as [ρₜ ρₛ].
+    unfold rbank_assert_t, rbank_assert_t_single in Haddr.
+    apply get_at_unfold in Hpre.
+    destruct Hpre as (loc & Hloc & Hmem).
+
+    eapply FTargetSteps.
+    - eexists. eapply exec_Iload; try eassumption.
+      + unfold get_at. rewrite Hloc. simpl_map. reflexivity.
+      + reflexivity.
+    - intros t Hstep.
+      inv Hstep as [ | | | ? ? ? ? ? ? ? ? ? ? ? ? ? Hget | | | | | ].
+      unfold get_at in Hget. rewrite Hloc in Hget.
+      simpl_map. inv Hget.
+      eexists. eapply H; auto. simp.
+      unfold get_at. now rewrite Hloc.
+  Qed.
+
+  Lemma source_store C Γ Φ j fₜ pcₜ i fₛ pcₛ :
+    ∀ pc dst src addr v old,
+    fₛ@pcₛ is <<{ !dst := src -> pc }>> ->
+    Γ @ dst ⇒ₛ addr ->
+    Γ @ src ⇒ₛ v ->
+    C | Γ ⊢ {{ addr →ₛ v }} fₜ @ pcₜ <{j, 1+i}= fₛ @ pc {{ Φ }} ->
+    C | Γ ⊢ {{ addr →ₛ old }} fₜ @ pcₜ <{j, i}= fₛ @ pcₛ {{ Φ }}.
+  Proof using Type.
+    intros pc dst src addr v old Hpc Haddr Hv H.
+    intros Ψ mt1 ms1 ? ? Hpre mt2 ms2 ? ? Hpost.
+
+    simp.
+    destruct Γ as [ρₜ ρₛ].
+    apply get_at_unfold in Hpre. destruct Hpre as (l & Hloc & Hmem).
+
+    eapply FSourceSteps.
+    - eapply exec_Istore; try eassumption.
+      unfold set_at, update_at. rewrite Hloc.
+      simpl_map.
+      rewrite (insert_union_l _ ms2).
+      rewrite (insert_union_r ∅ ms1).
+      + reflexivity.
+      + eapply map_disjoint_Some_l; eassumption.
+    - eapply H; auto.
+      + apply map_disjoint_insert_l. split; now eauto.
+      + unfold get_at. rewrite Hloc.
+        now rewrite (lookup_insert_eq ms1).
+      + decompose_map_disjoint.
+        apply map_disjoint_union_r. split; auto.
+        * solve_map_disjoint.
+        * apply map_disjoint_insert_r. split; eauto.
+          eapply map_disjoint_Some_r; eassumption.
+  Qed.
+
+  Lemma target_store C Γ Φ j fₜ pcₜ i fₛ pcₛ :
+    ∀ pc dst src addr v old,
+    fₜ@pcₜ is <<{ !dst := src -> pc }>> ->
+    Γ @ dst ⇒ₜ addr ->
+    Γ @ src ⇒ₜ v ->
+    C | Γ ⊢ {{ addr →ₜ v }} fₜ @ pc <{1+j, i}= fₛ @ pcₛ {{ Φ }} ->
+    C | Γ ⊢ {{ addr →ₜ old }} fₜ @ pcₜ <{j, i}= fₛ @ pcₛ {{ Φ }}.
+  Proof using Type.
+    intros pc dst src addr v old Hpc Haddr Hv H.
+    intros Ψ mt1 ms1 ? ? Hpre mt2 ms2 ? ? Hpost.
+
+    destruct Γ as [ρₜ ρₛ].
+    unfold rbank_assert_t, rbank_assert_t_single in Haddr, Hv.
+    apply get_at_unfold in Hpre. destruct Hpre as (l & Hloc & Hmem).
+
+    eapply FTargetSteps.
+    - eexists. eapply exec_Istore; try eassumption.
+      unfold set_at, update_at. rewrite Hloc.
+      simpl_map. reflexivity.
+    - intros t Hstep.
+      inv Hstep as [ | | | | ? ? ? ? ? ? ? ? ? ? ? ? ? ? Hm | | | | ].
+      unfold set_at, update_at in Hm. rewrite Hloc in Hm.
+      simpl_map.
+      rewrite (insert_union_l _ mt2) in Hm.
+      rewrite (insert_union_r ∅ mt1) in Hm by solve_map_disjoint.
+      inv Hm.
+
+      eexists. simp. apply H; auto.
+      + apply map_disjoint_insert_l. split; now auto.
+      + unfold get_at. rewrite Hloc.
+        now rewrite (lookup_insert_eq mt1).
+      + decompose_map_disjoint.
+        apply map_disjoint_union_r. split; auto.
+        * solve_map_disjoint.
+        * apply map_disjoint_insert_r. split; eauto.
+          eapply map_disjoint_Some_r; eassumption.
+  Qed.
+
+  Lemma source_if C Γ Φ j fₜ pcₜ i fₛ pcₛ :
+    ∀ pc_true pc_false reg v pc,
+    fₛ@pcₛ is <<{ if reg then goto pc_true else goto pc_false }>> ->
+    Γ @ reg ⇒ₛ v ->
+    (if (v =? 0)%Z then pc_true else pc_false) = pc ->
+    C | Γ ⊢ {{ ⌜⌝ }} fₜ @ pcₜ <{j, 1+i}= fₛ @ pc {{ Φ }} ->
+    C | Γ ⊢ {{ ⌜⌝ }} fₜ @ pcₜ <{j, i}= fₛ @ pcₛ {{ Φ }}.
+  Proof using Type.
+    intros pc_true pc_false reg v pc Hpc Hv Hnext_pc H.
+    intros Ψ ? ? ? ? Hpre ? ? ? ? Hpost. simp.
+
+    destruct Γ as [ρₜ ρₛ].
+    unfold rbank_assert_s, rbank_assert_s_single in Hv.
 
     eapply FSourceSteps.
     - econstructor; eassumption || reflexivity.
-    - now eapply Hsim.
+    - subst. now apply H.
   Qed.
 
-  Lemma target_load (C : Chain fsim_lfp) Q j fₜ pcₜ i fₛ pcₛ :
-    ∀ pc dst src addr v,
-    fₜ@pcₜ is <{ dst := !src -> pc }> ->
-    ⊨ src ⇒ₜ addr ->
-      addr →ₜ v ->
-      ⟦ dst ⇐ₜ v ⟧ C ⊢ ⟨fₜ @ pc, S j⟩ ≲ ⟨fₛ @ pcₛ, i⟩ {{ Q }} ->
-      C ⊢ ⟨fₜ @ pcₜ, j⟩ ≲ ⟨fₛ @ pcₛ, i⟩ {{ Q }}.
+  Lemma target_if C Γ Φ j fₜ pcₜ i fₛ pcₛ :
+    ∀ pc_true pc_false reg v pc,
+    fₜ@pcₜ is <<{ if reg then goto pc_true else goto pc_false }>> ->
+    Γ @ reg ⇒ₜ v ->
+    (if (v =? 0)%Z then pc_true else pc_false) = pc ->
+    C | Γ ⊢ {{ ⌜⌝ }} fₜ @ pc <{j, i}= fₛ @ pcₛ {{ Φ }} ->
+    C | Γ ⊢ {{ ⌜⌝ }} fₜ @ pcₜ <{j, i}= fₛ @ pcₛ {{ Φ }}.
   Proof using Type.
-    intros pc dst src addr v Hpc.
-    intros ρₜ ρₛ mₜ mₛ Hsrc Haddr [? [Hnew Hsim]] Ψ Hpost. simp.
+    intros pc_true pc_false reg v pc Hpc Hv Hnext_pc H.
+    intros Ψ ? ? ? ? Hpre ? ? ? ? Hpost. simp.
 
-    injection Hsrc as Hsrc.
-    injection Hnew as Hnew.
+    destruct Γ as [ρₜ ρₛ].
+    unfold rbank_assert_t, rbank_assert_t_single in Hv.
 
     eapply FTargetSteps.
     - eexists. econstructor; eassumption || reflexivity.
     - intros t Hstep. inv Hstep.
-      eexists. now apply Hsim.
+      eexists. now apply H.
   Qed.
 
-  Lemma source_store (C : Chain fsim_lfp) Q j fₜ pcₜ i fₛ pcₛ :
-    ∀ pc dst src addr v,
-    fₛ@pcₛ is <{ !dst := src -> pc }> ->
-    ⊨ src ⇒ₛ v ->
-      dst ⇒ₛ addr ->
-      ⟦ addr ←ₛ v ⟧ C ⊢ ⟨fₜ @ pcₜ, j⟩ ≲ ⟨fₛ @ pc, S i⟩ {{ Q }} ->
-      C ⊢ ⟨fₜ @ pcₜ, j⟩ ≲ ⟨fₛ @ pcₛ, i⟩ {{ Q }}.
+  Lemma frame C Γ Φ j fₜ pcₜ i fₛ pcₛ :
+    ∀ P Q,
+    C | Γ ⊢ {{ Q }} fₜ @ pcₜ <{j, i}= fₛ @ pcₛ {{ fun vₜ vₛ => Φ vₜ vₛ }} ->
+    C | Γ ⊢ {{ P ∗ Q }} fₜ @ pcₜ <{j, i}= fₛ @ pcₛ {{ fun vₜ vₛ => P ∗ Φ vₜ vₛ }}.
   Proof using Type.
-    intros pc dst src addr v Hpc.
-    intros ρₜ ρₛ mₜ mₛ Hsrc Haddr [? [Hnew Hsim]] Ψ Hpost. simp.
+    intros P Q H.
+    intros Ψ mt2 ms2 ? ? Hpre mt3 ms3 ? ? Hpost.
+    decompose_map_disjoint.
 
-    injection Hsrc as Hsrc.
-    injection Haddr as Haddr.
+    destruct Hpre as (mtP & mtQ & msP & msQ & ? & ? & ? & ? & Hp & Hq).
 
-    eapply FSourceSteps.
-    - econstructor; eassumption || reflexivity.
-    - now eapply Hsim.
+    unfold hoare in H. simp.
+
+    rewrite (map_empty_union mt2).
+    rewrite (map_empty_union ms2).
+
+    subst. decompose_map_disjoint.
+
+    rewrite (map_union_comm mtP mtQ) by auto.
+    rewrite (map_union_comm msP msQ) by auto.
+
+    rewrite <- (map_union_assoc mtQ mtP mt3).
+    rewrite <- (map_union_assoc msQ msP ms3).
+
+    rewrite <- (map_empty_union (mtQ ∪ (mtP ∪ mt3))).
+    rewrite <- (map_empty_union (msQ ∪ (msP ∪ ms3))).
+
+    rewrite ! (map_union_assoc ∅ _ _).
+
+    apply H.
+    - solve_map_disjoint.
+    - solve_map_disjoint.
+    - assumption.
+    - solve_map_disjoint.
+    - solve_map_disjoint.
+    - intros vₜ vₛ mt' ms' ? ? ?.
+      subst. decompose_map_disjoint.
+
+      rewrite (map_union_comm mtP mt3) by auto.
+      rewrite (map_union_comm msP ms3) by auto.
+
+      rewrite <- (map_union_assoc mt3 mtP mt').
+      rewrite <- (map_union_assoc ms3 msP ms').
+
+      apply Hpost.
+      + solve_map_disjoint.
+      + solve_map_disjoint.
+      + do 4 eexists. repeat split.
+        * solve_map_disjoint.
+        * solve_map_disjoint.
+        * assumption.
+        * assumption.
   Qed.
 
-  Lemma target_store (C : Chain fsim_lfp) Q j fₜ pcₜ i fₛ pcₛ :
-    ∀ pc dst src addr v,
-    fₜ@pcₜ is <{ !dst := src -> pc }> ->
-    ⊨ src ⇒ₜ v ->
-      dst ⇒ₜ addr ->
-      ⟦ addr ←ₜ v ⟧ C ⊢ ⟨fₜ @ pc, S j⟩ ≲ ⟨fₛ @ pcₛ, i⟩ {{ Q }} ->
-      C ⊢ ⟨fₜ @ pcₜ, j⟩ ≲ ⟨fₛ @ pcₛ, i⟩ {{ Q }}.
+  Lemma consequence C Γ Φ j fₜ pcₜ i fₛ pcₛ :
+    ∀ P P' Φ',
+    (⊨ P -* P') ->
+    C | Γ ⊢ {{ P' }} fₜ @ pcₜ <{j, i}= fₛ @ pcₛ {{ Φ' }} ->
+    (∀ vₜ vₛ, ⊨ Φ' vₜ vₛ -* Φ vₜ vₛ) ->
+    C | Γ ⊢ {{ P }} fₜ @ pcₜ <{j, i}= fₛ @ pcₛ {{ Φ }}.
   Proof using Type.
-    intros pc dst src addr v Hpc.
-    intros ρₜ ρₛ mₜ mₛ Hsrc Haddr [? [Hnew Hsim]] Ψ Hpost. simp.
+    intros P P' Φ' HP H HΦ.
+    intros Ψ mt2 ms2 ? ? Hpre mt3 ms3 ? ? Hpost.
 
-    injection Hsrc as Hsrc.
-    injection Haddr as Haddr.
-
-    eapply FTargetSteps.
-    - eexists. econstructor; eassumption || reflexivity.
-    - intros t Hstep. inv Hstep.
-      eexists. now apply Hsim.
+    simp. apply H; auto.
+    - rewrite <- (map_empty_union mt2).
+      rewrite <- (map_empty_union ms2).
+      apply HP; now auto.
+    - intros vₜ vₛ mt ms ? ? HΦ'.
+      apply Hpost; auto.
+      rewrite <- (map_empty_union mt).
+      rewrite <- (map_empty_union ms).
+      apply HΦ.
+      + solve_map_disjoint.
+      + solve_map_disjoint.
+      + assumption.
   Qed.
-
-  Lemma source_if (C : Chain fsim_lfp) Q j fₜ pcₜ i fₛ pcₛ :
-    ∀ pc_true pc_false reg v,
-    fₛ@pcₛ is <{ if reg then goto pc_true else goto pc_false }> ->
-    ⊨ reg ⇒ₛ v ->
-      C ⊢ ⟨fₜ @ pcₜ, j⟩ ≲ ⟨fₛ @ if (v =? 0)%Z then pc_true else pc_false, i⟩ {{ Q }} ->
-      C ⊢ ⟨fₜ @ pcₜ, j⟩ ≲ ⟨fₛ @ pcₛ, i⟩ {{ Q }}.
-  Proof using Type.
-    intros pc_true pc_false reg Hpc Hv.
-    intros ρₜ ρₛ mₜ mₛ Harg Hsim Ψ Hpost. simp.
-
-    injection Harg as Harg.
-
-    eapply FSourceSteps.
-    - econstructor; eassumption || reflexivity.
-    - now apply Hsim.
-  Qed.
-
-  Lemma target_if (C : Chain fsim_lfp) Q j fₜ pcₜ i fₛ pcₛ :
-    ∀ pc_true pc_false reg v,
-    fₜ@pcₜ is <{ if reg then goto pc_true else goto pc_false }> ->
-    ⊨ reg ⇒ₜ v ->
-      C ⊢ ⟨fₜ @ if (v =? 0)%Z then pc_true else pc_false, j⟩ ≲ ⟨fₛ @ pcₛ, i⟩ {{ Q }} ->
-      C ⊢ ⟨fₜ @ pcₜ, j⟩ ≲ ⟨fₛ @ pcₛ, i⟩ {{ Q }}.
-  Proof using Type.
-    intros pc_true pc_false reg Hpc Hv.
-    intros ρₜ ρₛ mₜ mₛ Harg Hsim Ψ Hpost. simp.
-
-    injection Harg as Harg.
-
-    eapply FTargetSteps.
-    - eexists. econstructor; eassumption || reflexivity.
-    - intros t Hstep. inv Hstep.
-      eexists. now apply Hsim.
-  Qed.
-
 End Rules.
