theories/Playground/SimTest.v
@@ -31,7 +31,7 @@ Section T.
       fn_name := "fact"%string;
       fn_regs := [n; addr];
       fn_entrypoint := 0;
-      fn_code := <{{
+      fn_code := <<{{
             0: result := #1 -> 1;
             1: !addr := result -> 2;
             2: if n then goto 6 else goto 3;
@@ -39,7 +39,7 @@ Section T.
             4: one := !addr -> 5;
             5: n := n - one -> 2;
             6: ret result;
-        }}>;
+        }}>>;
       fn_regs_no_dup := eq_refl;
     |}.
 
@@ -48,14 +48,14 @@ Section T.
       fn_name := "fact"%string;
       fn_regs := [n];
       fn_entrypoint := 0;
-      fn_code := <{{
+      fn_code := <<{{
             0: result := #1 -> 1;
             1: one := #1 -> 2;
             2: if n then goto 5 else goto 3;
             3: result := result * n -> 4;
             4: n := n - one -> 2;
             5: ret result;
-        }}>;
+        }}>>;
       fn_regs_no_dup := eq_refl;
     |}.
 
@@ -66,8 +66,8 @@ Section T.
     (sim Pₜ Pₛ (elem C) Φ j ft pct i fs pcs)
       (at level 1, ft at level 0, fs at level 0, no associativity).
 
-  Definition veq (vₜ vₛ : val) (mₜ mₛ: memory) :=
-    vₜ = vₛ.
+  (* Definition veq (vₜ vₛ : val) (mₜ mₛ: memory) := *)
+  (*   vₜ = vₛ. *)
 
   (* Haddr : get_reg addr ρₛ = v *)
   (* ρₜ : regmap *)
@@ -83,41 +83,41 @@ Section T.
   (* ============================ *)
   (* C ⊢ ⟨ fact_good @ 2, 2 ⟩ ≲ ⟨ fact_bad @ 2, 2 ⟩ {{veq}} (ρₜ, mₜ) (ρₛ, mₛ) *)
 
-  Lemma inv (C: Chain fsim_lfp) : ∀  loc,
-    ⊨ addr ⇒ₛ loc ->
-    result ₜ≈ₛ result ->
-    n ₜ≈ₛ n ->
-    one ⇒ₜ 1 ->
-    loc →ₛ 1 ->
-    C ⊢ ⟨fact_good @ 2, 0⟩ ≲ ⟨fact_bad @ 2, 0⟩ {{ veq }}.
-  Proof using Type.
-    intros loc.
-    intros ρₜ ρₛ mₜ mₛ Haddr Hres Hn Hone Hloc Ψ Hpost. simp.
-    injection Haddr as Haddr.
-    injection Hres as Hres.
-    injection Hn as Hn.
-    injection Hone as Hone.
+  (* Lemma inv (C: Chain fsim_lfp) : ∀  loc, *)
+  (*   ⊨ addr ⇒ₛ loc -> *)
+  (*   result ₜ≈ₛ result -> *)
+  (*   n ₜ≈ₛ n -> *)
+  (*   one ⇒ₜ 1 -> *)
+  (*   loc →ₛ 1 -> *)
+  (*   C ⊢ ⟨fact_good @ 2, 0⟩ ≲ ⟨fact_bad @ 2, 0⟩ {{ veq }}. *)
+  (* Proof using Type. *)
+  (*   intros loc. *)
+  (*   intros ρₜ ρₛ mₜ mₛ Haddr Hres Hn Hone Hloc Ψ Hpost. simp. *)
+  (*   injection Haddr as Haddr. *)
+  (*   injection Hres as Hres. *)
+  (*   injection Hn as Hn. *)
+  (*   injection Hone as Hone. *)
 
-    eapply @coind_rule.
-    intros C' j i CIH.
-    cut (C' ⊢ ⟨ fact_good @ 2, 0 ⟩ ≲ ⟨ fact_bad @ 2, 0 ⟩ {{veq}} ρₜ ρₛ mₜ mₛ).
-    {
-      intros H. unfold sim in H. simp.
-      eapply (@fsim_lfp_mono).
-      - eapply (H Ψ).
-        apply Hpost.
-      - destruct j.
-        + now right.
-        + left. simpl. lia.
-      - destruct i.
-        + now right.
-        + left. simpl. lia.
-    }
-    eapply source_if; try reflexivity.
-  (*   iRegUpdate. *)
+  (*   eapply @coind_rule. *)
+  (*   intros C' j i CIH. *)
+  (*   cut (C' ⊢ ⟨ fact_good @ 2, 0 ⟩ ≲ ⟨ fact_bad @ 2, 0 ⟩ {{veq}} ρₜ ρₛ mₜ mₛ). *)
+  (*   { *)
+  (*     intros H. unfold sim in H. simp. *)
+  (*     eapply (@fsim_lfp_mono). *)
+  (*     - eapply (H Ψ). *)
+  (*       apply Hpost. *)
+  (*     - destruct j. *)
+  (*       + now right. *)
+  (*       + left. simpl. lia. *)
+  (*     - destruct i. *)
+  (*       + now right. *)
+  (*       + left. simpl. lia. *)
+  (*   } *)
+  (*   eapply source_if; try reflexivity. *)
+  (* (*   iRegUpdate. *) *)
 
-    admit.
-  Admitted.
+  (*   admit. *)
+  (* Admitted. *)
 
   (*   unfold_bilogic. *)
   (*   simpl_memory by idtac. *)
