theories/RelLogic.v
@@ -1,1 +1,2 @@
 From RSL Require Export RelLogic.Logic.
+From RSL Require Export RelLogic.Memory.
