theories/RelLogic/Memory.v
@@ -1,0 +1,76 @@
+From RSL Require Import Prelude.
+
+From stdpp Require Import gmap.
+From RSL Require Import Commons.RegisterBank.
+
+Definition rbank : Type := regbank * regbank.
+
+Class RLogicTargetAssert (R V : Type) :=
+  rbank_assert_t : rbank -> R -> V -> Prop.
+
+Instance rbank_assert_t_single : RLogicTargetAssert _ _ :=
+  fun '(ρₜ, _) key val => get_reg ρₜ key = val.
+
+Instance rbank_assert_t_list : RLogicTargetAssert (list _) (list _) :=
+  fun '(ρₜ, _) keys vals => map (get_reg ρₜ) keys = vals.
+
+Definition rbank_update_t '((ρₜ, ρₛ) : rbank) key f : rbank :=
+  (update_reg ρₜ key f, ρₛ).
+
+Definition rbank_set_t Γ key val : rbank :=
+  rbank_update_t Γ key (fun _ => val).
+
+Class RLogicSourceAssert (R V : Type) :=
+  rbank_assert_s : rbank -> R -> V -> Prop.
+
+Instance rbank_assert_s_single : RLogicSourceAssert _ _ :=
+  fun '(_, ρₛ) key val => get_reg ρₛ key = val.
+
+Instance rbank_assert_s_list : RLogicSourceAssert (list _) (list _) :=
+  fun '(_, ρₛ) keys vals => map (get_reg ρₛ) keys = vals.
+
+Definition rbank_update_s '((ρₜ, ρₛ) : rbank) key f : rbank :=
+  (ρₜ, update_reg ρₛ key f).
+
+Definition rbank_set_s Γ key val : rbank :=
+  rbank_update_s Γ key (fun _ => val).
+
+Notation "Γ @ r '⇒ₜ' v" :=
+  (rbank_assert_t Γ r%nat v%Z)
+    (at level 60, no associativity).
+
+Notation "Γ @ r '⇒ₛ' v" :=
+  (rbank_assert_s Γ r%nat v%Z)
+    (at level 60, no associativity).
+
+Notation "'⟦' r '⇐ₜ' v '⟧' Γ" :=
+  (rbank_set_t Γ r%nat v%Z)
+    (at level 20, Γ at level 20, right associativity).
+
+Notation "'⟦' r '⇐ₛ' v '⟧' Γ" :=
+  (rbank_set_s Γ r%nat v%Z)
+    (at level 20, Γ at level 20, right associativity).
+
+Notation "'⟦' r '⇐ₜ' 'λ' v '.' f '⟧' Γ" :=
+  (rbank_update_t Γ r%nat (fun v => f))
+    (at level 20, v binder, Γ at level 20, right associativity).
+
+Notation "'⟦' r '⇐ₛ' 'λ' v '.' f '⟧' Γ" :=
+  (rbank_update_s Γ r%nat (fun v => f))
+    (at level 20, v binder, Γ at level 20, right associativity).
+
+Notation "'⟦' r '⇐ₜ' 'fun' v '.' f '⟧' Γ" :=
+  (rbank_update_t Γ r%nat (fun v => f))
+    (at level 20, v binder, Γ at level 20, right associativity).
+
+Notation "'⟦' r '⇐ₛ' 'fun' v '.' f '⟧' Γ" :=
+  (rbank_update_s Γ r%nat (fun v => f))
+    (at level 20, v binder, Γ at level 20, right associativity).
+
+Notation "'⟦' rt '⇐ₜ' vt ',' rs '⇐ₛ' vs '⟧' Γ" :=
+  (rbank_update_t (rbank_update_s Γ rs%nat vs%Z) rt%nat vt%Z)
+    (at level 20, Γ at level 20, right associativity).
+
+Notation "'⟦' rs '⇐ₛ' vs ',' rt '⇐ₜ' vt '⟧' Γ" :=
+  (rbank_update_t (rbank_update_s Γ rs%nat vs%Z) rt%nat vt%Z)
+    (at level 20, Γ at level 20, right associativity).
