theories/Simulations/Equiv/GSimToEAltSim.v
@@ -4,7 +4,6 @@ From Coinduction Require Import all.
 
 From RSL Require Import Commons.OrdTree.
 
-From RSL Require Import Simulations.Commons.
 From RSL Require Import Simulations.FreeSim.
 
 From RSL Require Import Simulations.Equiv.GSim.
